## Question 3

$E = 6a - b + 25$

#### Proof: That E is a loop measure

(1) Let $n \geq 1$ be arbitrary. We claim that $E_{n+1} \leq E_n-1$.

(2) If the loop condition is being checked for the n+1st time, then it was previously checked for the n-th time and evaluated to true. When line 3 is reached for the n-th time, either $a_n > 0$ or $a_n \leq 0$. Proceed by cases.

(3) Case 1: $a_n > 0$. Then the condition on line 3 evaluates to true, so lines 4 and 5 are executed and line 7 is skipped. In line 4, $a_{n+1}$ is assigned the value $a_n-4$. In line 5, $b_{n+1}$ is assigned the value $b_n-20$. So, 

$$E_{n+1} = 6a_{n+1} - b_{n+1} + 25$$

$$= 6a_{n} - 24 - b_{n} + 20 + 25$$

$$= 6a_{n} - b_{n} + 25 - 4$$

$$= E_{n} - 4 < E_n-1$$

(4) Case 2: $a_n \leq 0$. Then the condition on line 3 evaluates to false, so lines 4 and 5 are skipped and line 7 is executed. In line 7, $b_{n+1}$ is assigned the value $b_n+3$ and $a_{n+1}$ is not modified, so $a_{n+1} = a_n$. Now,  

$$E_{n+1} = 6a_{n+1} - b_{n+1} + 25$$

$$= 6a_{n} - b_{n} - 3 + 25$$

$$= E_{n} - 3 < E_n - 1$$

(5) By (3) and (4), in all cases, $E_{n+1} \leq E_n-1$.

(6) Now, suppose that $E \leq 0$. We claim that the loop condition evauluates to false. That is, $a \leq 0 \land b \geq 5$.

(7) By the given loop invariant, $a \geq -3$, and $b \leq 7 \implies -b \geq -7$, which together imply that 

$$E = 6a -b + 25\space \geq \space 6(-3) -7 +25 = 0$$

By supposition, $E \leq 0$, so $E = 0$. However, this can only occur if $a = -3$ and $b = 7$, so $a \leq 0$ and $b \geq 5$, as needed. Therefore, when $E \leq 0$, the loop evaluates to false.

(8) Thus, by (5) and (7), $E = 6a - b + 25$ is a loop measure.
