## Question 4

```
1. //Pre: n >= 1
2. x <-- 2*n
3. sum <-- 0
4. //LoopInv: x is even
5. while(x > 0)
6.      y <-- 0
7.      while(y < x)
8.          sum <-- sum + 3*y
9.          y <-- y + 1
10.     x <-- x - 2
```

### (a) Find $f(n)$, the number of **steps** that this program executes as a function of $n$.

For the outer loop, $x$ starts at $2n$ and decreases by $2$ until it it executes its final iteration when $x=2$, since $x$ is even from the loop invariant. So, $x=2n, 2n-2, 2n-4, ..., 4, 2$. Let $k=x/2$, then $k$ starts at $n$ and decreases by $1$ until $k=1$. Since addition is commutative, the sum from $n$ decreasing until $1$ is equal to the sum from $1$ increasing until $n$. 

For the inner loop, $y$ starts at $0$ and increases by $1$ until it it executes its final iteration when $y=x-1=2k-1$ since $x = 2k$. So, $y=1, 2, 3, ..., 2k-2, 2k-1$. So, the number of steps exectuted by the inner loop is

$$\sum_{y=0}^{2k-1}(3) + 1 = 6k+1$$

, since lines 7, 8, and 9 are executed each iteration, and then we add $1$ for the final time the loop condition is checked and evaluates to false.

Then, the number of steps executed by the entire program is

$$\sum_{k=1}^{n}(3 + 6k + 1) + 1 + 2$$

Since lines 5, 6, and 10 are executed once per outer loop iteration, the inner loop is executed once per outer loop iteration, and then add the final check of the loop condition when it evaluates to false as well as when lines 2 and 3 are executed at the beginning of the program. We can further simplify this to 

$$= 6 \sum_{k=1}^{n}(k) + \sum_{k=1}^{n}(4) + 3$$
$$= \frac{6n(n+1)}{2} + 4n + 3$$
$$= \frac{6n^2 + 6n + 8n + 6}{2}$$
$$= 3n^2 + 7n + 3$$

Thus, a function $f(n)$ that calculates the number of steps that this program executes as a function of n is

$$f(n) = 3n^2 + 7n + 3$$

### (b) 

The value of the variable sum starts at $0$, then it is only modified within the inner loop where it is set to the value $sum = sum + 3y$. 
