## Question 2

### (a)

#### Proof:
(1) We wish to disprove $\exists a > 1,\space \exists M > 0,\space \forall x \in \mathbb{R} (a^x \geq M)$, where $a,M \in \mathbb{R}$. It suffices to prove the negation. Which is:  

$$\forall a > 1,\space \forall M > 0,\space \exists x\ (a^x < M) $$

(2) Let $a,M \in \mathbb{R}$ be arbitrary, such that $a > 1$ and $M > 0$.

(3) Let $x = \log_a(M-1)$

(4) Then we have,

$$a^x = a^{\log_a(M-1)} = M-1 < M$$
$$\implies a^x < M$$

as needed.

(5) Thus, since $a,M \in \mathbb{R}$, were both arbitrary, we conclude that $\forall a > 1,\space \forall M > 0,\space \exists x\ (a^x < M)$. 

### (b)

#### Proof:
(1) We wish to prove $\forall x \in \mathbb{R},\space \forall y \in \mathbb{R}\space ((y-x > 1)\implies (\exists n \in \mathbb{Z}\space (x < n < y)))$. 

(2) Let $x,y \in \mathbb{R}$ be arbitrary, and assume that $y-x > 1$.

(3) Notice that either $x \not \in \mathbb{Z}$, or $x \in \mathbb{Z}$. We proceed by cases.

(4) Note that from (2), $y - x > 1 \implies x+1 < y$

(5) Case 1: If $x \not \in \mathbb{Z}$, let $n = \lceil x \rceil$. 

Now, $n= \lceil x \rceil > x\space$, so, $\space n > x$. And by (4), $n = \lceil x \rceil < x+1 < y$. So, $n < y$. 

Therefore, $x < n < y$, as needed.

(6) Case 2: If $x \in \mathbb{Z}$, let $n= x+1$. 

Now, $n=x+1 > x\space$, so, $\space n > x$. And by (4), $n=x+1 < y\space$, so $\space n < y$.

Therefore, $x < n < y$, as needed.

(7) In either case, since $x$ and $y$ were arbitrary, $x < n < y$, as needed. Thus, 
$$\forall x \in \mathbb{R},\space \forall y \in \mathbb{R}\space ((y-x > 1)\implies (\exists n \in \mathbb{Z}\space (x < n < y)))$$


