## Question 4

#### Proof:
(1) Define the sequence of numbers $a_n$ for all positive integers as follows:
$$a_1=-10,\space a_2=2, \space and \quad \forall n \geq 3, \space a_n=a_{n-1}+12a_{n-2}$$

(2) Let P(n) be the predicate that $a_n=2(-3)^n-4^n$. We will prove using strong mathematical induction that $\forall n \in \mathbb{N}$, P(n).

(3) Base Case: When $n=1$ we have $a_1=-10$ and $2(-3)^1-4^1 = -10$. Thus P(1) is true.

(4) Base Case: When $n=2$ we have $a_2=2$ and $2(-3)^2-4^2 = 18-16=2$. Thus P(2) is true.

(5) Induction Step: Let $n \geq 2$ be arbitrary, and assume that $\forall k \leq n$, 

$$a_{k}=2(-3)^{k}-4^{k}$$

We will prove P(n+1), which states

$$a_{n+1}=2(-3)^{n+1}-4^{n+1}$$

(6) We have, 

$$a_{n+1} = a_{n}+12a_{n-1}$$

$$a_{n+1} = 2(-3)^{n}-4^{n}+12(2(-3)^{n-1}-4^{n-1})\quad , by\quad I.H$$

$$a_{n+1} = 2(-3)^{n}-4^{n}+24(-3)^{n-1}-12(4)^{n-1}$$

$$a_{n+1} = 2(-3)^{n}-4^{n}-8(-3)^{n}-3(4)^{n}$$

$$a_{n+1} = -6(-3)^{n}-4(4)^{n}$$

$$a_{n+1} = 2(-3)^{n+1}-4^{n+1}$$

as needed.

(7) Thus, since P(1) and P(2) are true, and $\forall k \leq n$, P(k) $\implies$ P(n+1), by the principle of strong mathematical induction, we conclude that $\forall n \in \mathbb{N}, \space a_n = 2(-3)^n-4^n$.
